# Chapter 5.3

### 12. Show that  $Cov(\bar x, s^2) = \frac{v_3}{n}$, \ where $\ v_3 = E[x-E(x)]^3$, $\ E(\bar x) = \mu$

Intuition: We first note that the highest term of R.H.S. is 3, then we try to do some operations so that the highest term of the L.H.S. is also 3. 

First, we have

$$
Cov(\bar x, s^2) = E(\bar x \sdot s^2)-E(\bar x)E(s^2)
$$

We note that both terms have 3 as the highest term, so we just try to combine 2 terms together. Then we have

$$
E(\bar x \sdot s^2)-E(\bar x)E(s^2) = E(\bar x \sdot s^2)-\mu E(s^2)= E[(\bar x-\mu)s^2]
$$

Then, we try to simplify $(\bar x-\mu)s^2$  in order to get more information. The trick is that we want all x transform into $x - \mu$, because after doing that, we have all the term about x having the format as x-E(x) just like v3. so we get

$$
\begin{split}
(\bar x-\mu)s^2 &= (\bar x-\mu)\frac{1}{n-1}(\sum^n_{i=1}x^2_i-n \bar x^2)\\
&= (\bar x-\mu)\frac{1}{n-1}[\sum^n_{i=1}(x_i-\mu)^2-n(\bar x -\mu)^2]
\end{split}
$$

Then, we can find the expectation of them separately. 

First,

$$
\begin{split}
E(\bar x-\mu)[\sum^n_{i=1}(x_i-\mu)^2]
&= \sum^n_{i=1}E[(\bar x-\mu)(x_i-\mu)^2] \\

\end{split}
$$

Then, we have 

$$
E[(\bar x-\mu)(x_i-\mu)^2] =
\frac{1}{n}E(x_i-\mu)^3-\sum_{i \not = j}E[(x_j-\mu)(x_i-\mu)^2]
$$

note that $x_i, \ x_j$  are independent, then we have $E(x_j-\mu)E(x_i-\mu)^2 = 0$. Thus, we have

$$
E[(\bar x-\mu)(x_i-\mu)^2] =
\frac{1}{n}E(x_i-\mu)^3 = \frac{v_3}{n}
$$

Second,

$$
E(\bar x- \mu)^3 = \frac{1}{n^3}\sum^n_{i=1}E(x_i-\mu)^3=\frac{v_3}{n^2}
$$

Combine them together, we get the answer

### 22. Find the distribution  of  $x_{(1)}$ and  $x_{(n)}$, given P(X=k)

For this type of question, the intuition is similar. We just find $P(X \leq k)$ and $P(X \geq k)$.

Since we have $P(x_{(1)}=k) = P(x_{(1)}\geq k) - P(x_{(1)}\geq k+1)$ 

and $P(x_{(n)}=k) = P(x_{(n)} \leq k)-P(x_{(n)} \leq k-1)$

but actually, we can use formula to solve this question.
